Fix subtype relation, add surface language syntax
Added base type
modeling and base type translation to expression. Subtype relation is now fixed using those. Finished the pending proof too. Also added the surface language syntax except dereferencing.

src/semantic_rules.v
@@ -364,7 +364,7 @@ Inductive subtype
     forall var τb e₁ e₂,
       ty_valid Γ Φ (TSet var τb e₁) ->
       ty_valid Γ Φ (TSet var τb e₂) ->
-      eval ((var , TBase τb) :: Γ) Γv Φ ι (EImp e₁ e₂) (EBool true) -> (* TODO ide valahogy a var-nak τb összes értékét is oda kéne adni (egyesével), hogy tudjon működni az eval *)
+      ∀ (c : (base_to_set τb)), eval ((var , TBase τb) :: Γ) ((var , make_expr τb c) :: Γv) Φ ι (EImp e₁ e₂) (EBool true) ->
       subtype Γ Γv Φ ι (TSet var τb e₁) (TSet var τb e₂)
   | SSetBase :
     forall var τb e,
@@ -373,7 +373,7 @@ Inductive subtype
   | SBaseSet :
     forall var τb e,
       ty_valid Γ Φ (TSet var τb e) ->
-      eval ((var , TBase τb) :: Γ) Γv Φ ι e (EBool true) -> (* TODO ide valahogy a var-nak τb összes értékét is oda kéne adni (egyesével), hogy tudjon működni az eval *)
+      ∀ (c : (base_to_set τb)), eval ((var , TBase τb) :: Γ) ((var , make_expr τb c) :: Γv) Φ ι e (EBool true) ->
       subtype Γ Γv Φ ι (TBase τb) (TSet var τb e)
   | SFun :
     forall τ₁ τ₁' τ₂ τ₂',
@@ -399,7 +399,7 @@ Inductive subtype
 Lemma set_sub_test : forall Γ Γv Φ ι, subtype Γ Γv Φ ι (TSet "x" BBool (ENot (EVar "x"))) (TSet "x" BBool (EBool true)).
 Proof.
 intros.
-apply SSet.
+eapply SSet.
 apply VSet.
 apply PNot.
 apply PVar.
@@ -407,19 +407,26 @@ simpl. reflexivity.
 simpl. reflexivity.
 apply VSet.
 apply PBool.
-(* apply eval_imp with (e₁ := ENot (EVar "x")) (e₂ := EBool true) (* (b₁ := ?? true és false is lehet...) *) (b₂ := true). *)
-Admitted.
+simpl.
+apply eval_imp with (e₁ := ENot (EVar "x")) (e₂ := EBool true) (b₁ := true) (b₂ := true).
+apply eval_not with (b := false).
+eapply eval_var.
+simpl; reflexivity.
+simpl; reflexivity.
+apply eval_bool.
+Qed.
 
 (* two equivalent sets *)
 Lemma set_sub_test_without_var_use : forall Γ Γv Φ ι, subtype Γ Γv Φ ι (TSet "x" BBool (ENot (EBool false))) (TSet "x" BBool (EBool true)).
 Proof.
 intros.
-apply SSet.
+apply SSet with (c := true).
 apply VSet.
 apply PNot.
 apply PBool.
 apply VSet.
 apply PBool.
+simpl.
 apply eval_imp with (e₁ := ENot (EBool false)) (e₂ := EBool true) (b₁ := true) (b₂ := true).
 apply eval_not with (e := EBool false) (b := false).
 apply eval_bool.
@@ -430,7 +437,7 @@ Qed.
 Lemma set_sub_test_without_var_use2 : forall Γ Γv Φ ι, subtype Γ Γv Φ ι (TSet "x" BBool (ENot (EBool true))) (TSet "x" BBool (EBool true)).
 Proof.
 intros.
-apply SSet.
+apply SSet with (c := true).
 apply VSet.
 apply PNot.
 apply PBool.
@@ -442,7 +449,23 @@ apply eval_bool.
 apply eval_bool.
 Qed.
 
-
+Lemma base_sub_set_test : forall Γ Γv Φ ι, subtype Γ Γv Φ ι (TBase BBool) (TSet "x" BBool (EOr (EBool true) (EVar "x"))).
+Proof.
+intros.
+eapply SBaseSet.
+apply VSet.
+apply POr.
+apply PBool.
+apply PVar.
+simpl; reflexivity.
+simpl; reflexivity.
+simpl.
+apply eval_or with (b₁ := true) (b₂ := false).
+apply eval_bool.
+eapply eval_var.
+simpl; reflexivity.
+simpl; reflexivity.
+Qed.
 
 
 
